buffered_io.v
@@ -1,0 +1,460 @@
+From iris.algebra Require Import auth.
+From iris_io Require Import lang rules list.
+From iris_io Require Import petrinet adequacy.
+From iris.proofmode Require Import tactics.
+From iris.program_logic Require Import weakestpre lifting.
+From iris.base_logic Require Import viewshifts.
+
+Section buffered_io.
+  Context `{heapIG Σ, petrinetIG Σ}.
+
+  Definition beep_tag := 1%positive.
+  Definition write_tag := 2%positive.
+
+  Definition write :=
+    Rec
+      (Case
+         (Var 1)
+         Plang.Unit
+         (Seq
+            (IO (IOtag write_tag) (Fst (Var 0)))
+            (LetIn (Snd (Var 0)) (App (Var 2) (Var 0)))
+         )
+      ).
+
+  Lemma write_closed : ∀ f, write.[f] = write.
+  Proof. done. Qed.
+
+  Lemma write_eq :
+    write =
+    Rec
+      (Case
+         (Var 1)
+         Plang.Unit
+         (Seq
+            (IO (IOtag write_tag) (Fst (Var 0)))
+            (LetIn (Snd (Var 0)) (App (Var 2) (Var 0)))
+         )
+      ).
+  Proof. trivial. Qed.
+
+  Hint Rewrite write_closed : autosubst.
+
+  Typeclasses Opaque write.
+  Global Opaque write.
+
+  Fixpoint write_prim_ p c q :=
+    match c with
+    | [] => p = q
+    | v :: c' =>
+      ∃ s, ThePetriNet (IOTr p write_tag v Plang.UnitV s)
+           ∧ write_prim_ s c' q
+    end.
+
+  Definition write_ P c Q :=
+    (∃ p q R, (P ={⊤}=> Token p ∗ R)
+                ∗ ⌜write_prim_ p c q⌝ ∗ (Token q ∗ R ={⊤}=> Q))%I.
+
+  Lemma write_extend p c q v q' :
+    write_prim_ p c q → ThePetriNet (IOTr q write_tag v Plang.UnitV q') →
+    write_prim_ p (c ++ [v]) q'.
+  Proof.
+    revert p q v; induction c => p q v Hc Hv.
+    - simpl in *; simplify_eq.
+      eexists _; repeat split; eauto.
+    - destruct Hc as [s [Hs Hw]]; eexists _; eauto.
+  Qed.
+
+  Lemma wp_write p c q :
+    write_prim_ p c q →
+    {{{ Token p }}}
+      (App write (of_val (of_list c)))
+    {{{RET  UnitV; Token q }}}.
+  Proof.
+  iIntros (Hwr Φ) "Hp HΦ".
+  iInduction c as [|x c] "IH" forall (p q Hwr).
+  - simpl in *; subst.
+    rewrite write_eq.
+    iApply wp_pure_step_later; auto.
+    rewrite -write_eq.
+    iNext. asimpl.
+    iApply wp_pure_step_later; auto.
+    asimpl. iNext. iApply wp_value.
+    by iApply "HΦ"; iFrame.
+  - destruct Hwr as [s [Hs Hwr]]; simpl in *.
+    rewrite write_eq.
+    iApply wp_pure_step_later; auto.
+    rewrite -write_eq.
+    iNext. asimpl.
+    iApply wp_pure_step_later; auto.
+    asimpl. iNext.
+    iApply (wp_bind (fill [SeqCtx _])).
+    iApply (wp_bind (fill [IORCtx (IOtagV _)])).
+    iApply wp_pure_step_later; auto.
+    iNext. iApply wp_value; simpl.
+    iApply (wp_petrinet_io with "Hp"); eauto.
+    iIntros "!> Hs".
+    iApply wp_pure_step_later; auto.
+    iNext. asimpl.
+    iApply (wp_bind (fill [LetInCtx _])).
+    iApply wp_pure_step_later; auto.
+    iNext. iApply wp_value; simpl.
+    iApply wp_pure_step_later; auto.
+    iNext. asimpl.
+    iApply ("IH" with "[] Hs"); eauto.
+  Qed.
+
+  Definition putchar l :=
+    Lam
+      (If
+         (BinOp Eq (#n 1000) (App list_length (Load l.[ren (+1)])))
+         (Seq (LetIn (Load l.[ren (+1)]) (App write (Var 0)))
+              (Store l.[ren (+1)] (InjR (Pair (Var 0) (InjL Plang.Unit)))))
+         (LetIn (Load l.[ren (+1)])
+                (Store l.[ren (+2)] (App (App snoc (Var 0)) (Var 1))))).
+
+  Lemma putchar_closed l :
+    ∀ f, (putchar l).[f] = (putchar l.[f]).
+  Proof. by intros f; rewrite /putchar; asimpl. Qed.
+
+  Hint Rewrite putchar_closed : autosubst.
+
+  Lemma putchar_eq l :
+    putchar l =
+    Lam
+      (If (BinOp Eq (#n 1000) (App list_length (Load l.[ren (+1)])))
+          (Seq (LetIn (Load l.[ren (+1)]) (App write (Var 0)))
+               (Store l.[ren (+1)] (InjR (Pair (Var 0) (InjL Plang.Unit)))))
+          (LetIn (Load l.[ren (+1)])
+                 (Store l.[ren (+2)] (App (App snoc (Var 0)) (Var 1))))).
+  Proof. trivial. Qed.
+
+  Typeclasses Opaque putchar.
+  Global Opaque putchar.
+
+  Definition buffer_token l p :=
+    (∃ c p0, l ↦ (of_list c) ∗ Token p0 ∗ ⌜write_prim_ p0 c p⌝)%I.
+
+  Definition putchar_ l p1 v p2 :=
+    (∃ p'1 p'2 R,
+      (p1 ={⊤}=> buffer_token l p'1 ∗ R)
+      ∧ ⌜ThePetriNet (IOTr p'1 write_tag v Plang.UnitV p'2)⌝
+      ∧ (buffer_token l p'2 ∗ R ={⊤}=> p2) )%I.
+
+  Lemma wp_putchar l P v Q :
+    {{{ P ∗ putchar_ l P v Q }}}
+      App (putchar (Loc l)) (of_val v)
+    {{{RET UnitV; Q }}}.
+  Proof.
+    iIntros (Φ) "[HP Hpc] HΦ".
+    iDestruct "Hpc" as (p1 p2 R) "(#Hp1 & % & #Hp2)".
+    iMod ("Hp1" with "HP") as "[HP HR]".
+    iDestruct "HP" as (c q) "(Hl & Hq & %)".
+    rewrite putchar_eq.
+    iApply wp_pure_step_later; trivial.
+    iNext. asimpl.
+    iApply (wp_bind (fill [IfCtx _ _])).
+    iApply (wp_bind (fill [BinOpRCtx _ (#nv _)])).
+    rewrite list_length_eq.
+    iApply (wp_bind (fill [AppRCtx (RecV _)])); simpl.
+    rewrite -list_length_eq.
+    iApply (wp_load with "Hl"); iIntros "!> Hl".
+    iApply wp_list_length; auto.
+    iNext. iIntros (w Hw); subst.
+    iApply wp_pure_step_later; trivial.
+    rewrite /binop_eval.
+    destruct PeanoNat.Nat.eq_dec.
+    - iApply wp_value. iNext.
+      iApply wp_pure_step_later; trivial.
+      iNext.
+      iApply (wp_bind (fill [SeqCtx _])).
+      iApply (wp_bind (fill [LetInCtx _])).
+      iApply (wp_load with "Hl"); iIntros "!> Hl /=".
+      iApply wp_pure_step_later; trivial.
+      iNext. asimpl.
+      iApply (wp_write with "Hq"); eauto.
+      iNext. iIntros "Hpt1"; simplify_eq.
+      iApply wp_pure_step_later; trivial.
+      iNext.
+      iApply wp_fupd.
+      iApply (wp_store with "Hl"); iIntros "!> Hl /=".
+      iMod ("Hp2" with "[$HR Hpt1 Hl]") as "HQ".
+      { iExists [_], _; iFrame; simpl; eauto. }
+      by iModIntro; iApply "HΦ"; iFrame.
+    - iApply wp_value.
+      iNext.
+      iApply wp_pure_step_later; trivial.
+      iNext.
+      iApply (wp_bind (fill [LetInCtx _])).
+      iApply (wp_load with "Hl"); iIntros "!> Hl /=".
+      iApply wp_pure_step_later; trivial. iNext. asimpl.
+      iApply (wp_bind (fill [StoreRCtx (LocV _)])).
+      iApply wp_snoc; auto.
+      iNext. iIntros (w ?); simplify_eq; simpl.
+      iApply wp_fupd.
+      iApply (wp_store with "Hl"); iIntros "!> Hl /=".
+      iMod ("Hp2" with "[$HR Hq Hl]") as "HQ".
+      { iExists (_ ++ [_]), _; iFrame; simpl; eauto using write_extend. }
+      by iModIntro; iApply "HΦ"; iFrame.
+  Qed.
+
+  Definition flush l :=
+    Seq (LetIn (Load l) (App write (Var 0)))
+        (Store l (InjL Plang.Unit)).
+
+  Lemma flush_closed l : ∀ f, (flush l).[f] = flush l.[f].
+  Proof. done. Qed.
+
+  Hint Rewrite flush_closed : autosubst.
+
+  Lemma flush_eq l :
+    flush l =
+    Seq (LetIn (Load l) (App write (Var 0)))
+        (Store l (InjL Plang.Unit)).
+  Proof. trivial. Qed.
+
+  Typeclasses Opaque flush.
+  Global Opaque flush.
+
+  Definition flush_ l P Q :=
+    (∃ p' R, (P ={⊤}=> buffer_token l p' ∗ R)
+               ∗ (Token p' ∗ l ↦ (InjLV UnitV) ∗ R ={⊤}=> Q))%I.
+
+  Lemma wp_flush l P Q :
+    {{{ P ∗ flush_ l P Q }}} flush (Loc l) {{{ RET UnitV; Q }}}.
+  Proof.
+    iIntros (Φ) "[HP Hfl] HΦ".
+    iDestruct "Hfl" as (p' R) "(#Hp & #HQ)".
+    iMod ("Hp" with "HP") as "[HP HR]".
+    iDestruct "HP" as (c q) "(Hl & Hq & %)".
+    rewrite flush_eq.
+    iApply (wp_bind (fill [SeqCtx _])).
+    iApply (wp_bind (fill [LetInCtx _])).
+    iApply (wp_load with "Hl"); iIntros "!> Hl /=".
+    iApply wp_pure_step_later; trivial.
+    iNext. asimpl.
+    iApply (wp_write with "Hq"); eauto.
+    iNext. iIntros "Hp'"; subst.
+    iApply wp_pure_step_later; trivial.
+    iNext.
+    iApply wp_fupd.
+    iApply (wp_store with "Hl"); iIntros "!> Hl /=".
+    iMod ("HQ" with "[$HR $Hp' $Hl]") as "Hq".
+    by iModIntro; iApply "HΦ"; iFrame.
+  Qed.
+
+  Definition beep := IO (IOtag beep_tag) Plang.Unit.
+
+  Lemma beep_closed : ∀ f, beep.[f] = beep.
+  Proof. done. Qed.
+
+  Definition beep_ P Q :=
+    (∃ p q R,
+        (P ={⊤}=> Token p ∗ R)
+          ∗ ⌜ThePetriNet (IOTr p beep_tag Plang.UnitV Plang.UnitV q)⌝
+          ∗ (Token q ∗ R ={⊤}=> Q)
+    )%I.
+
+  Lemma wp_beep P Q :
+    {{{ P ∗ beep_ P Q }}} beep {{{ RET UnitV; Q }}}.
+  Proof.
+    iIntros (Φ) "[HP Hbp] HΦ".
+    iDestruct "Hbp" as (p q R) "(#Hp & % & #Hq)".
+    iMod ("Hp" with "HP") as "[Htp HR]".
+    iApply wp_fupd.
+    iApply (wp_petrinet_io with "Htp"); eauto.
+    iNext. iIntros "Htq".
+    iMod ("Hq" with "[$Htq $HR]") as "HQ".
+    by iModIntro; iApply ("HΦ" with "[$HQ]").
+  Qed.
+
+  Definition start :=
+    LetIn
+      (Alloc (InjL Plang.Unit))
+      (Seq beep (Seq (App (putchar (Var 0)) (#n 1)) (flush (Var 0)))).
+
+  Lemma wp_start P1 P2 P3 :
+    {{{ P1 ∗ beep_ P1 P2 ∗ write_ P2 [(#nv 1)] P3 }}}
+      start
+    {{{RET UnitV; P3 }}}.
+  Proof.
+    iIntros (Φ) "(Hp1 & #Hbp & #Hwr) HΦ".
+    iDestruct "Hwr" as (p2 p3 R) "(Hp2 & Hwr & Hp3)"; simpl in *.
+    iDestruct "Hwr" as %[s [Hwr ?]]; simpl in *; simplify_eq.
+    iApply (wp_bind (fill [LetInCtx _])).
+    iApply (wp_alloc); auto; iNext; iIntros (l) "Hl /=".
+    iApply wp_pure_step_later; trivial.
+    iNext. asimpl.
+    iApply (wp_bind (fill [SeqCtx _])).
+    iApply (wp_beep with "[Hp1]")%I.
+    { by iFrame "#". }
+    iNext. iIntros "HP2". simpl.
+    iApply wp_pure_step_later; trivial.
+    iNext.
+    iApply (wp_bind (fill [SeqCtx _])).
+    iApply (wp_putchar _ (P2 ∗ l ↦ InjLV UnitV) (#nv _)
+                       (buffer_token l p3 ∗ R)%I
+              with "[HP2 Hl] [HΦ]").
+    { iFrame. iExists _, _, R.
+      repeat iSplit; eauto.
+      - iIntros "!# [HP2 Hl]".
+        iMod ("Hp2" with "HP2") as "[HP2 HR]".
+        iFrame. iModIntro. iExists [], _; iFrame; eauto.
+      -  by iIntros "!# [$ $]". }
+    iNext. iIntros "[Hbt HR] /=".
+    iApply wp_pure_step_later; trivial.
+    iNext.
+    iApply wp_fupd.
+    iApply (wp_flush _ (buffer_token l p3 ∗ R) (Token p3 ∗ l ↦ InjLV UnitV ∗ R)
+              with "[$Hbt $HR]")%I; eauto.
+    { iExists _, R. iSplit.
+      - by iIntros "!# [$ $]".
+      - by iIntros "!# ($ & $ & $)". }
+    iNext. iIntros "(HP3 & Hl & HR)".
+    iMod ("Hp3" with "[$HP3 $HR]") as "HP3".
+    by iApply "HΦ".
+  Qed.
+
+
+End buffered_io.
+
+Inductive bufferedIO_places :=
+  BIO_Start
+| BIO_beep_done
+| BIO_write_done.
+
+Global Instance bufferedIO_places_eqdec :
+  EqDecision bufferedIO_places.
+Proof. solve_decision. Qed.
+
+Instance bufferedIO_petri_placesC : PlacesC :=
+  {| Places := bufferedIO_places |}.
+
+Inductive bufferedIO_petri : PetriNet :=
+| BIO_beepTR :
+    bufferedIO_petri (IOTr BIO_Start beep_tag UnitV UnitV BIO_beep_done)
+| BIO_writeTR :
+    bufferedIO_petri (IOTr BIO_beep_done write_tag (#nv 1) UnitV BIO_write_done).
+
+Lemma singVAL_eq p q V : singVAL p ⊎ V = singVAL q → p = q ∧ V = (λ x, 0).
+Proof.
+  intros Heq.
+  split.
+  - pose proof (equal_f Heq p) as Heq'.
+    revert Heq'. rewrite /singVAL /ValPlus /=.
+    repeat destruct decide; done.
+  - extensionality z.
+    pose proof (equal_f Heq z) as Heq'.
+    pose proof (equal_f Heq p) as Heq''.
+    revert Heq' Heq''. rewrite /singVAL /ValPlus /=.
+    repeat destruct decide; subst; auto with omega; try done.
+Qed.
+
+Lemma Valuation_unit V : V ⊎ (λ _, 0) = V.
+Proof. extensionality z. rewrite /ValPlus; omega. Qed.
+
+Ltac trvial_petri := match goal with
+| H : bufferedIO_petri (SplitTr ?p _ _) |- _ => destruct p; inversion H
+| H : bufferedIO_petri (JoinTr ?p _ _) |- _ => destruct p; inversion H
+| H : bufferedIO_petri (NoOpTr ?p _) |- _ => destruct p; inversion H
+end.
+
+Lemma Traces_bufferedIO_petri τ :
+  Traces bufferedIO_petri (singVAL BIO_Start) τ →
+  τ = [] ∨ τ = [(beep_tag, UnitV, UnitV)] ∨
+  τ = [(beep_tag, UnitV, UnitV); (write_tag, (#nv 1), UnitV)].
+Proof.
+  inversion 1; eauto; try trvial_petri.
+  edestruct singVAL_eq; eauto; simplify_eq.
+  match goal with
+  | H: bufferedIO_petri (IOTr BIO_Start _ _ _ _) |- _ => inversion H; subst
+  end.
+  repeat match goal with
+         | H : context [(λ _, 0)] |- _ =>
+           rewrite Valuation_unit in H
+         end.
+  match goal with
+  | H: Traces bufferedIO_petri (singVAL BIO_beep_done) _ |- _ =>
+    inversion H; subst; eauto; try trvial_petri
+  end.
+  right; right.
+  edestruct singVAL_eq; eauto; simplify_eq.
+  match goal with
+  | H: bufferedIO_petri (IOTr BIO_beep_done _ _ _ _) |- _ => inversion H; subst
+  end.
+  repeat match goal with
+         | H : context [(λ _, 0)] |- _ =>
+           rewrite Valuation_unit in H
+         end.
+  match goal with
+  | H: Traces bufferedIO_petri (singVAL BIO_write_done) _ |- _ =>
+    inversion H; subst; eauto; try trvial_petri
+  end.
+  edestruct singVAL_eq; eauto; simplify_eq.
+  match goal with
+  | H: bufferedIO_petri (IOTr BIO_write_done _ _ _ _) |- _ => inversion H; subst
+  end.
+Qed.
+
+Lemma app_not_nil {A} (l l' : list A) x :
+  l ++ x :: l' ≠ [].
+Proof. induction l; auto. Qed.
+
+Lemma bufferedIO_petri_ResultDet :
+  ResultDet (Traces bufferedIO_petri (singVAL BIO_Start)).
+Proof.
+  intros t v v' v'' τ τ' τ'' Hτ Hτ'.
+  apply Traces_bufferedIO_petri in Hτ;
+    apply Traces_bufferedIO_petri in Hτ'.
+  destruct τ as [|? []]; simpl in *; intuition; simplify_eq; auto.
+  exfalso; eapply app_not_nil; eauto.
+Qed.
+
+Theorem wp_closed_start
+        `{heapIPreIOG Σ}
+        `{inG Σ (authUR (ofe_funUR (λ p : Places, natUR)))} :
+  (|={⊤}=> ∃ γio, let _ := make_heapIG γio in
+                 |={⊤}=> ∃ _ : petrinetIG Σ,
+     FullIO (Traces bufferedIO_petri (singVAL BIO_Start))
+            ∗ WP start {{v, ⌜v = UnitV⌝ }})%I.
+Proof.
+  iIntros "".
+  pose (Traces bufferedIO_petri (singVAL BIO_Start)) as ios.
+  iMod (@own_alloc _ io_monoid _
+                   (● Excl' (ios : leibnizC ioSpec) ⋅
+                      ◯ Excl' (ios : leibnizC ioSpec))) as (γio) "[HFI HOI]";
+    first done.
+  iModIntro. iExists _. pose (make_heapIG γio). iFrame.
+  iMod (PetriNetInv_alloc with "HOI") as (γpn) "[#HPi HOV]".
+  { apply bufferedIO_petri_ResultDet. }
+  pose ({| γPN := γpn; ThePetriNet := bufferedIO_petri|}) as PN.
+  iModIntro. iExists PN.
+  set (tk := @Token bufferedIO_petri_placesC _ _ _).
+  iAssert (tk BIO_Start) with "[$HOV]" as "HOS"; first done.
+  iApply (wp_start (tk BIO_Start) (tk BIO_beep_done) (tk BIO_write_done)
+            with "[$HOS]").
+  { iSplit.
+    - iExists _, _, True%I; repeat iSplit.
+      + by iIntros "!# $".
+      + iPureIntro; econstructor.
+      + by iIntros "!# [$ _]".
+    - iExists BIO_beep_done, BIO_write_done, True%I; repeat iSplit.
+      + by iIntros "!# $".
+      + iPureIntro. eexists _; simpl; split; eauto using bufferedIO_petri.
+      + by iIntros "!# [$ _]". }
+  by iIntros "!> _".
+Qed.
+
+Theorem start_safe :
+  fully_erased_safe start (Traces bufferedIO_petri (singVAL BIO_Start)).
+Proof.
+  pose (#[IoΣ; petrinetΣ]) as Σ.
+  apply (adequacy Σ _ ((λ _, True))%I).
+  { apply Traces_prefix_closed. }
+  intros Hig.
+  iIntros "".
+  iMod (wp_closed_start) as (γio) "Hlm".
+  iMod ("Hlm") as (HIG) "[HFIO HWP]".
+  iModIntro; iExists _; iFrame.
+  by iApply @wp_wand_l; iFrame.
+Qed.
