list.v
@@ -1,0 +1,214 @@
+From iris_io Require Export lang rules.
+From iris.proofmode Require Import tactics.
+From iris.program_logic Require Import weakestpre lifting.
+
+
+Fixpoint of_list (l : list val) :=
+  match l with
+    [] => InjLV Plang.UnitV
+  | v :: l' => InjRV (PairV v (of_list l'))
+  end.
+
+Global Instance of_list_inj : Inj eq eq of_list.
+Proof.
+  intros x.
+  induction x => y Heq; first by destruct y.
+  destruct y; first done.
+  inversion Heq; subst.
+  f_equal. by apply IHx.
+Qed.
+
+
+Definition append :=
+  Rec
+    (Lam
+       (Case
+          (Var 2) (Var 1)
+          (InjR
+             (Pair (Fst (Var 0)) (App (App (Var 2) (Snd (Var 0))) (Var 1)))
+          )
+       )
+    ).
+
+Lemma append_closed f : append.[f] = append.
+Proof. by asimpl. Qed.
+
+Hint Rewrite append_closed : autosubst.
+
+Lemma append_eq :
+  append = Rec
+             (Lam
+                (Case
+                   (Var 2) (Var 1)
+                   (InjR
+                      (Pair (Fst (Var 0)) (App (App (Var 2) (Snd (Var 0))) (Var 1)))
+                   )
+                )
+             ).
+Proof. trivial. Qed.
+
+Typeclasses Opaque append.
+Global Opaque append.
+
+Lemma wp_append `{heapIG Σ} l l' :
+  {{{True}}} (App (App append (of_val (of_list l))) (of_val (of_list l')))
+          {{{w, RET w; ⌜w = of_list (l ++ l')⌝}}}.
+Proof.
+  iIntros (Φ) "_ HΦ".
+  iLöb as "IH" forall (Φ l).
+  rewrite append_eq.
+  iApply (wp_bind (fill [AppLCtx _])).
+  iApply wp_pure_step_later; auto.
+  rewrite -append_eq.
+  iNext. asimpl.
+  iApply wp_value. simpl.
+  iApply wp_pure_step_later; auto.
+  iNext. asimpl.
+  destruct l.
+  - simpl. iApply wp_pure_step_later; eauto.
+    iNext. asimpl. iApply wp_value. by iApply "HΦ".
+  - simpl. iApply wp_pure_step_later; auto.
+    iNext. asimpl.
+    iApply (wp_bind (fill [InjRCtx])).
+    iApply (wp_bind (fill [PairLCtx _])).
+    iApply wp_pure_step_later; auto.
+    iNext; iApply wp_value. simpl.
+    iApply (wp_bind (fill [PairRCtx _])).
+    rewrite append_eq.
+    iApply (wp_bind (fill [AppRCtx (RecV _); AppLCtx _])).
+    iApply wp_pure_step_later; auto.
+    iNext; iApply wp_value; simpl.
+    iApply wp_wand_r; iSplitR.
+    { iApply ("IH" $! (λ s, ⌜s = of_list (l ++ l')⌝))%I. iNext.
+        by iIntros (w Hw); subst w. }
+    simpl.
+    iIntros (w) "%"; subst; simpl.
+    do 2 iApply wp_value.
+      by iApply "HΦ".
+Qed.
+
+Definition snoc :=
+  Rec
+    (Lam
+       (Case
+          (Var 2) (InjR (Pair (Var 1) (InjL Plang.Unit)))
+          (InjR
+             (Pair (Fst (Var 0)) (App (App (Var 2) (Snd (Var 0))) (Var 1)))
+          )
+       )
+    ).
+
+Lemma snoc_closed f : snoc.[f] = snoc.
+Proof. by asimpl. Qed.
+
+Hint Rewrite snoc_closed : autosubst.
+
+Lemma snoc_eq :
+  snoc =
+  Rec
+    (Lam
+       (Case
+          (Var 2) (InjR (Pair (Var 1) (InjL Plang.Unit)))
+          (InjR
+             (Pair (Fst (Var 0)) (App (App (Var 2) (Snd (Var 0))) (Var 1)))
+          )
+       )
+    ).
+Proof. trivial. Qed.
+
+Typeclasses Opaque snoc.
+Global Opaque snoc.
+
+Lemma wp_snoc `{heapIG Σ} l u :
+  {{{True}}} (App (App snoc (of_val (of_list l))) (of_val u))
+          {{{w, RET w; ⌜w = of_list (l ++ [u])⌝}}}.
+Proof.
+  iIntros (Φ) "_ HΦ".
+  iLöb as "IH" forall (Φ l).
+  rewrite snoc_eq.
+  iApply (wp_bind (fill [AppLCtx _])).
+  iApply wp_pure_step_later; auto.
+  rewrite -snoc_eq.
+  iNext. asimpl.
+  iApply wp_value. simpl.
+  iApply wp_pure_step_later; auto.
+  iNext. asimpl.
+  destruct l.
+  - simpl. iApply wp_pure_step_later; eauto.
+    iNext. asimpl. iApply wp_value. by iApply "HΦ".
+  - simpl. iApply wp_pure_step_later; auto.
+    iNext. asimpl.
+    iApply (wp_bind (fill [InjRCtx])).
+    iApply (wp_bind (fill [PairLCtx _])).
+    iApply wp_pure_step_later; auto.
+    iNext; iApply wp_value. simpl.
+    iApply (wp_bind (fill [PairRCtx _])).
+    rewrite snoc_eq.
+    iApply (wp_bind (fill [AppRCtx (RecV _); AppLCtx _])).
+    iApply wp_pure_step_later; auto.
+    iNext; iApply wp_value; simpl.
+    iApply wp_wand_r; iSplitR.
+    { iApply ("IH" $! (λ s, ⌜s = of_list (l ++ [u])⌝))%I. iNext.
+        by iIntros (w Hw); subst w. }
+    simpl.
+    iIntros (w) "%"; subst; simpl.
+    do 2 iApply wp_value. by iApply "HΦ".
+Qed.
+
+Definition list_length :=
+  Rec
+    (Case
+       (Var 1)
+       (#n 0)
+       (BinOp Plang.Add (#n 1) (App (Var 1) (Snd (Var 0))))
+    ).
+
+Lemma list_length_closed f : list_length.[f] = list_length.
+Proof. by asimpl. Qed.
+
+Hint Rewrite list_length_closed : autosubst.
+
+Lemma list_length_eq :
+  list_length =
+  Rec
+    (Case
+       (Var 1)
+       (#n 0)
+       (BinOp Plang.Add (#n 1) (App (Var 1) (Snd (Var 0))))
+    ).
+Proof. trivial. Qed.
+
+Typeclasses Opaque list_length.
+Global Opaque list_length.
+
+Lemma wp_list_length `{heapIG Σ} l :
+  {{{True}}} (App list_length (of_val (of_list l)))
+          {{{w, RET w; ⌜w = (#nv (length l))⌝}}}.
+Proof.
+  iIntros (Φ) "_ HΦ".
+  iLöb as "IH" forall (Φ l).
+  rewrite list_length_eq.
+  iApply wp_pure_step_later; auto.
+  rewrite -list_length_eq.
+  iNext. asimpl.
+  destruct l.
+  - simpl. iApply wp_pure_step_later; eauto.
+    iNext. asimpl. iApply wp_value. by iApply "HΦ".
+  - simpl. iApply wp_pure_step_later; auto.
+    iNext. asimpl.
+    iApply (wp_bind (fill [BinOpRCtx _ (#nv _)])).
+    rewrite list_length_eq.
+    iApply (wp_bind (fill [AppRCtx (RecV _)])).
+    rewrite -list_length_eq.
+    iApply wp_pure_step_later; auto.
+    iNext; iApply wp_value; simpl.
+    rewrite -list_length_eq.
+    iApply wp_wand_r; iSplitR.
+    { iApply ("IH" $! (λ s, ⌜s = #nv (length l)⌝))%I. iNext.
+        by iIntros (w Hw); subst w. }
+    simpl.
+    iIntros (w) "%"; subst; simpl.
+    iApply wp_pure_step_later; auto.
+    iNext.
+    iApply wp_value. by iApply "HΦ".
+Qed.
